module polymorphism where

open import Agda.Primitive public

id : (A : Set) â†’ A â†’ A
id A x = x

-- No Girard paradoxes
-- So no Type:Type
-- So no self-application
{-
-- Setâ‚ != Set
id-id : (A : Set) â†’ A â†’ A
id-id = id ((A : Set) â†’ A â†’ A) id
-}

idâ‚ : (A : Setâ‚) â†’ A â†’ A
idâ‚ A x = x

idâ‚-id : (A : Set) â†’ A â†’ A
idâ‚-id = idâ‚ ((A : Set) â†’ A â†’ A) id

{-
-- Setâ‚‚ != Setâ‚
idâ‚-idâ‚ : (A : Setâ‚) â†’ A â†’ A
idâ‚-idâ‚ = idâ‚ ((A : Setâ‚) â†’ A â†’ A) idâ‚
-}

idâ‚‚ : (A : Setâ‚‚) â†’ A â†’ A
idâ‚‚ A x = x

idâ‚‚-idâ‚ : (A : Setâ‚) â†’ A â†’ A
idâ‚‚-idâ‚ = idâ‚‚ ((A : Setâ‚) â†’ A â†’ A) idâ‚

{-

 idâ‚ƒ
 idâ‚„
 idâ‚…

 .
 .
 .

-}

-- how do we get from id-n to id-(n+1) ?
id-Lift : âˆ€ {n} â†’ ((A : Set n) â†’ A â†’ A) â†’ ((A : Set (lsuc n)) â†’ A â†’ A)
id-Lift id-n = Î» A x â†’ x

-- what would be the limit of repeated application of id-Lift?
-- something like "(A : Set Ï‰) â†’ A â†’ A"
-- we can't do that, but with universe-polymorphism we can form
-- something equivalent:

idâˆ : âˆ€ Î± â†’ (A : Set Î±) â†’ A â†’ A
idâˆ Î± A x = x

-- pseudo-self-application: 
idâˆ-idâˆ : âˆ€ Î± â†’ (A : Set Î±) â†’ A â†’ A
idâˆ-idâˆ Î± = idâˆ (lsuc Î±) ((A : Set Î±) â†’ A â†’ A) (idâˆ Î±)

idâˆ' : âˆ€ {Î±} {A : Set Î±} â†’ A â†’ A
idâˆ' x = x

-- and with the polymorphism arguments made implicit, it looks
-- like regular self-application:
idâˆ'-idâˆ' : âˆ€ {Î±} {A : Set Î±} â†’ A â†’ A
idâˆ'-idâˆ' = idâˆ' idâˆ' 

data â„• : Set where
 ğ•« : â„•
 ğ•¤ : â„• â†’ â„•

add : â„• â†’ â„• â†’ â„•
add ğ•« y = y
add (ğ•¤ x) y = ğ•¤ (add x y) 

mul : â„• â†’ â„• â†’ â„•
mul ğ•« y = ğ•«
mul (ğ•¤ x) y = add y (mul x y)

fac : â„• â†’ â„•
fac ğ•« = (ğ•¤ ğ•«)
fac (ğ•¤ x) = mul (ğ•¤ x) (fac x)

almost-fac : (â„• â†’ â„•) â†’ (â„• â†’ â„•)
almost-fac f ğ•« = (ğ•¤ ğ•«)
almost-fac f (ğ•¤ x) = mul (ğ•¤ x) (f x)

{-
Y : âˆ€ {Î±} â†’ {A : Set Î±} â†’ (âˆ€ {Î²} â†’ {B : Set Î²} â†’ (A â†’ A) â†’ (A â†’ A)) â†’ A â†’ A
Y {Î±} {A} f = f (Y f)
-}

Y : (âˆ€ Î± â†’ (A : Set Î±) â†’ A â†’ A) â†’ (âˆ€ Î± â†’ (A : Set Î±) â†’ A â†’ A)
Y x Î± = x (lsuc Î±) ((A : Set Î±) â†’ A â†’ A) (x Î±)

Y' : (âˆ€ Î± â†’ (A : Set Î±) â†’ A â†’ A) â†’ (âˆ€ Î± â†’ (A : Set Î±) â†’ A â†’ A)
Y' x Î± =  

